\lecture{23}{Monday 24 February 2025}{02-24-25 Lecture}

-Midterm: Next Friday in class.

Limsup and Liminf

\begin{definition} 
	Let $\left( a_n \right) $ be a bounded sequence. Define the sequence $\left( y_n \right) $ as
	\begin{align}
		y_n = \sup \{a_k | k \ge n\} 
	\end{align}
	Then we have that $y_1, \ge y_2 \ge  y_3 \ge \ldots$ and  $\left( y_n \right) $ is a decreasing bounded sequence. Thus it cconverges by MCT. Define
	\begin{align}
		\lim_{} \sup a_n = \lim_{} y_n
	\end{align}
	Similarly define the sequence $\left( z_n \right) $ where
	\begin{align}
		z_n = \text{inf}\{a_k | k \ge n\} 
	\end{align}
	Therefore $z_1 \le z_2 \le z_3 < \ldots$ and $\left( z_n \right) $ is an increasing bounded sequence. Therefore it converges my MCT. Define
	\begin{align}
		\lim_{} \text{ inf } a_n = \lim_{} z_n
	\end{align}
\end{definition}

\begin{eg}
	$a_n = \left( -1 \right)^{n} \left( 1 + \frac{1}{n} \right) $ 
	\begin{align}
		a_ 1 = \left( -1 \right) \left( 1+\frac{1}{1} \right) = -1 - 1 \\
		a_2 = 1 \left( 1 + \frac{1}{2} \right) = 1 + \frac{1}{2} \\
		a_3 = -1\left( 1 + \frac{1}{3} \right) = -1 -\frac{1}{3} \\
		a_4 = 1 \left( 1 + \frac{1}{4} \right) = 1 + \frac{1}{4} \\
		a_5 = -1\left( 1 + \frac{1}{5} \right)  = -1 - \frac{1}{5}
	\end{align}
	So we have 
	\begin{align}
		y_1 = 1 + \frac{1}{2} \\
		y_2 = 1 + \frac{1}{2} \\
		y_3 = 1 + \frac{1}{4} \\
		y_4 = 1 + \frac{1}{4} \\
		y_5 = 1 + \frac{1}{6} \\
		y_6 = 1 + \frac{1}{6}
	\end{align}
	Therefore $\lim_{} y_n = 1$, thus $\lim_{} \sup a_n = 1$
	\begin{align}
		z_1 = 1 - 1\\
		z_2 = -1 -\frac{1}{3} \\
		z_3 = -1 -\frac{1}{3} \\
		z_4 = -1 -\frac{1}{5} \\
		z_5 = -1 -\frac{1}{5}
	\end{align}
	Therefore $\lim_{} z_n = -1$ and $\lim_{} \text{ inf } a_n = -1$
\end{eg}

\begin{eg}
	$a_n = \left( -1 \right)^{n} = -1, 1, -1, 1, \ldots$	

	\begin{align}
		\lim_{} \sup = 1 \\
		\lim_{} \text{ inf } = -1 \\
	\end{align}
\end{eg}

\begin{theorem}
	Let $\left( a_n \right)$ be a bounded sequence. The $\lim_{} \text{ inf } a_n \le \lim_{} \sup a_n$. Moreover, $\lim_{} \text{ inf } a_n = \lim_{} \sup a_n$ if and only if $\lim_{} a_n$ exists. In this case we have $\lim_{} \text{ inf } a_n = \lim_{} \sup a_n = \lim_{} a_n$
\end{theorem}

\begin{proof}
	\begin{enumerate}
		\item Observe that 
			\begin{align}
				\text{inf}\{a_k | k \ge 0\} \le \sup \{a_k | k \ge n\} 
			\end{align}
		Therefore $z_n \le y_n$ because $\lim_{} z_n = \lim_{} \text{inf } a_n$ and $\lim_{} y_n = \lim_{} \sup a_n$, therefore $\lim_{} \text{inf } a_n \le \lim_{} \sup a_n$.
		\item Assume that $\lim_{} \text{inf } a_n = \lim_{} \sup a_n = a$. We want to show that $\lim_{} a_n = a$. Let $\e > 0$ be given $\exists N_1 \in \N$ such that $\forall n \ge N_1$
			\begin{align}
				\left|z_n - a\right| < \e \implies a - \e < z_n < a + \e
			\end{align}
		Similarly, $\exists N_2 \in \N$ such that $\forall n \ge N_2$ 
		\begin{align}
			\left|y_n - a\right| < \e \implies a - \e < y_n < a + \e
		\end{align}
		Let $N = \text{max} \{N_1, N_2\} $. Therefore for all $n \ge N$ we have 
		\begin{align}
			a-\e < z_n \le a_n \le y_n \le a + \e \\
			\implies a - \e < a_n < a + \e \\
			\implies \left|a_n - a\right| < \e
		\end{align}
		Hence $\lim_{} a_n = a$. We want to show that $\lim_{} \text{inf } a_n = \lim_{} \sup a_n = a$. Let $\e > 0$ be given. Therefore $\exists N \in \N$ such that $\forall n \ge N$ we have
		\begin{align}
			\left|a_n - a\right| < \frac{\e}{2} \implies a - \frac{\e}{2} < a_n < a + \frac{\e}{2}
		\end{align}
		Now for all $n \ge N$ we have
		\begin{align}
			y_n = \sup \{a_k | k \ge n\} \implies a - \frac{\e}{2} \le y_n \le a + \frac{\e}{2} \\
			\implies \left|y_n - a\right| < \e
		\end{align}
		Therefore, $\lim_{} \sup a_n = a$. Similarly for all $n \ge N$ 
		\begin{align}
			z_n = \text{inf } \{a_k | k \ge n\} \implies a - \frac{\e}{2} \le z_n \le a + \frac{\e}{2} \implies \left|z_n - a\right| < \e \implies \lim_{} \text{inf } a_n = a
		\end{align}
	\end{enumerate}
\end{proof}

\begin{definition}
	Let $\left( a_n \right) $ be a seqience we say that $\lim_{} a_n = \inf$, if for any $M > 0$, $\exists N \in  \N$ such that $\forall n \ge N$ we have
	\begin{align}
		a_n > M
	\end{align}
	(we define $\lim_{} a_n = -\inf$ in a similar fashion).
\end{definition}

\begin{eg}
	Let $a_n = n^{2} + 1$. Prove that $\lim_{} a_n = \inf$
\end{eg}

\begin{proof}
	Let $M > 0$ be given. Choose $N \in  \N$ such that
	\begin{align}
		N > M
	\end{align}
	Then for all $n \ge  N$ we have
	\begin{align}
		n \ge N \implies n^{2} + 1 \ge N > M \\
		\implies n^{2} + 1 > M
	\end{align}
	Hence proved.
\end{proof}










